coq/ZF/Notation/Eval.v
@@ -1,0 +1,10 @@
+Declare Scope ZF_Notation_Eval_scope.
+Open    Scope ZF_Notation_Eval_scope.
+
+Require Import ZF.Set.Core.
+
+Class Eval (v:Type) := { eval : v -> U -> U }.
+
+Notation "F ! a" := (eval F a)
+  (at level 0, no associativity) : ZF_Notation_Eval_scope.
+
